

Lecture 11 Scribe: Transformation of Random Variables

February 10, 2026

Niharika Ashar

AU ID: AU2440175

Instructor: Dhaval Patel, PhD (Associate Professor)

SEAS – Ahmedabad University, Ahmedabad, Gujarat, India

1 Outline and Learning Objective

1.1 Topics in this lecture

1. **Transformation of Random Variables:** learning transformation techniques for random variables.
2. **Function of Two Random Variables:** joint transformations and derived distributions.
3. **Illustrative Example:** detailed derivation for the case $Z = X + Y$.

1.2 Assumption / setup stated in the outline

Assumption: the PDF of the original RV (e.g., $f_X(x)$) is known *a priori*; the goal is how to find the PDF of the new transformed RV (e.g., $f_Y(y)$).

1.3 Noted example transformations (as written on the outline slide)

$$Z_1 = X + Y, \quad Z_2 = X - Y, \quad Z_3 = \frac{X}{Y}, \quad Z_4 = \sqrt{X^2 + Y^2}.$$

2 Transformation of One Random Variable: $Y = g(X)$

2.1 Definitions and notation (as used on the slides)

A transformation is defined by

$$Y = g(X).$$

CDF notation: $F_Y(y)$ and $F_X(x)$.

PDF notation: $f_Y(y)$ and $f_X(x)$.

The slides proceed via **Step S1 (CDF)** then **Step S2 (differentiate w.r.t. y)**.

2.2 Assumption / condition: monotonicity

The slide distinguishes monotonic cases:

- **Monotonically increasing** case
- **Monotonically decreasing** case

2.3 Case A: $g(\cdot)$ is monotonically increasing

Step S1 (CDF method)

$$F_Y(y) = \Pr(Y \leq y) = \Pr(g(X) \leq y) = \Pr(X \leq g^{-1}(y)) = F_X(g^{-1}(y)).$$

Step S2 (Differentiate w.r.t. y)

$$f_Y(y) = \frac{d}{dy} [F_X(g^{-1}(y))] = f_X(g^{-1}(y)) \cdot \frac{d}{dy} (g^{-1}(y)).$$

Let $x = g^{-1}(y)$:

$$f_Y(y) = f_X(x) \left. \frac{dx}{dy} \right|_{x=g^{-1}(y)}.$$

2.4 Case B: $g(\cdot)$ is monotonically decreasing

Step S1 (CDF method)

$$F_Y(y) = \Pr(Y \leq y) = \Pr(X \geq g^{-1}(y)) = 1 - F_X(g^{-1}(y)).$$

Step S2 (Differentiate w.r.t. y)

$$f_Y(y) = \left. \frac{f_X(x)}{\left| \frac{dy}{dx} \right|} \right|_{x=g^{-1}(y)}.$$

S3 note: change the limits for y (determine valid y -range from the mapping).

3 Worked Example: $X \sim \text{Uniform}(-1, 1)$, $Y = \sin\left(\frac{\pi x}{2}\right)$

3.1 Given (from the example slide)

- X is uniform on $(-1, 1)$.
- Transformation:

$$Y = g(x) = \sin\left(\frac{\pi x}{2}\right).$$

- PDF of X :

$$f_X(x) = \begin{cases} \frac{1}{2}, & -1 < x < 1, \\ 0, & \text{otherwise.} \end{cases}$$

- Objective: find $f_Y(y)$.

3.2 Step-by-step solution (as shown)

Step 1: Invert the transformation

$$y = \sin\left(\frac{\pi x}{2}\right) \Rightarrow x = \frac{2}{\pi} \sin^{-1}(y).$$

Step 2: Differentiate x w.r.t. y

$$\frac{dx}{dy} = \frac{2}{\pi} \cdot \frac{1}{\sqrt{1-y^2}}.$$

Step 3: Apply the transformation formula

$$f_Y(y) = f_X(x) \cdot \left| \frac{dx}{dy} \right|.$$

Substitute $f_X(x) = \frac{1}{2}$:

$$f_Y(y) = \frac{1}{2} \cdot \frac{2}{\pi} \cdot \frac{1}{\sqrt{1-y^2}} = \frac{1}{\pi\sqrt{1-y^2}}.$$

Step 4: Determine the valid range of y from endpoints

- At $x = -1$: $y = \sin\left(-\frac{\pi}{2}\right) = -1$
- At $x = 1$: $y = \sin\left(\frac{\pi}{2}\right) = 1$

So the support is $-1 < y < 1$ (otherwise 0).

3.3 Final answer (as presented)

$$f_Y(y) = \begin{cases} \frac{1}{\pi\sqrt{1-y^2}}, & -1 < y < 1, \\ 0, & \text{otherwise.} \end{cases}$$

4 Function of Two Random Variables: Example Setup ($Z = X + Y$)**4.1 Problem statements listed on the slide**

For $Z = X + Y$, the slide lists:

1. Find the PDF of Z : $f_Z(z)$.
2. Find $f_Z(z)$ if X and Y are independent.
3. Let $X \sim N(0, 1)$ and $Y \sim N(0, 1)$; prove that $Z \sim N(0, 2)$.
4. If X and Y are exponential RVs with parameter λ , find $f_Z(z)$.

5 Detailed Derivation: CDF setup for $Z = X + Y$ via Region Integration**5.1 Definition of Z and CDF start**

$$Z = X + Y, \quad F_Z(z) = \Pr(Z \leq z) = \Pr(X + Y \leq z).$$

5.2 Region description and the “strip” integrals

Using the joint pdf $f_{XY}(x, y)$ and the boundary line $x + y = z$:

(A) Horizontal strip (H-strip) form

$$F_Z(z) = \int_{-\infty}^{\infty} \int_{-\infty}^{z-y} f_{XY}(x, y) dx dy.$$

(B) Vertical strip form

$$F_Z(z) = \int_{-\infty}^{\infty} \int_{-\infty}^{z-x} f_{XY}(x, y) \, dy \, dx.$$

End of Lecture 11 scribe.